LowStar.Modifies: expose lemmas about loc_unused_in

ulib/LowStar.Modifies.fst
@@ -278,15 +278,9 @@ let does_not_contain_addr_elim = MG.does_not_contain_addr_elim
 
 let modifies_only_live_addresses = MG.modifies_only_live_addresses
 
-val loc_not_unused_in (h: HS.mem) : GTot loc
 let loc_not_unused_in = MG.loc_not_unused_in _
 
-val loc_unused_in (h: HS.mem) : GTot loc
 let loc_unused_in = MG.loc_unused_in _
-
-val live_loc_not_unused_in (#t: Type) (b: B.buffer t) (h: HS.mem) : Lemma
-  (requires (B.live h b))
-  (ensures (loc_not_unused_in h `loc_includes` loc_buffer b))
 
 let live_loc_not_unused_in #t b h =
   B.unused_in_equiv b h;
@@ -296,10 +290,6 @@ let live_loc_not_unused_in #t b h =
   MG.loc_includes_trans (loc_not_unused_in h) (loc_addresses false (B.frameOf b) (Set.singleton (B.as_addr b))) (loc_buffer b);
   ()
 
-val unused_in_loc_unused_in (#t: Type) (b: B.buffer t) (h: HS.mem) : Lemma
-  (requires (B.unused_in b h))
-  (ensures (loc_unused_in h `loc_includes` loc_buffer b))
-
 let unused_in_loc_unused_in #t b h =
   B.unused_in_equiv b h;
   Classical.move_requires (MG.addr_unused_in_does_not_contain_addr h) (B.frameOf b, B.as_addr b);
@@ -307,6 +297,9 @@ let unused_in_loc_unused_in #t b h =
   loc_includes_addresses_buffer false (B.frameOf b) (Set.singleton (B.as_addr b)) b;
   MG.loc_includes_trans (loc_unused_in h) (loc_addresses false (B.frameOf b) (Set.singleton (B.as_addr b))) (loc_buffer b);
   ()
+
+let modifies_address_liveness_insensitive_unused_in =
+  MG.modifies_address_liveness_insensitive_unused_in cls
 
 
 let cloc_cls = cls
